src/rocq/Syntax/DynamicTypes.v
@@ -50,10 +50,12 @@ Set Elimination Schemes.
 (*  NOTE: to cut down on clutter, we coerce dtyp_base to dtyp *)
 Coercion DTYPE_Base : dtyp_base >-> dtyp.
 
+(* [Defined], not [Qed]: [eval_int_op] and friends branch on this test, so
+   it must compute for their [iptr]/[bit_int] instantiations to reduce. *)
 Lemma dtyp_base_eq_dec : forall (t1 t2 : dtyp_base), {t1 = t2} + {t1 <> t2}.
 Proof.
   repeat decide equality.
-Qed.
+Defined.
 
 Ltac dec_dtyp :=
   match goal with
